add copy-, fix arrow typing rule

theories/logrel/copying.v
@@ -1,21 +1,33 @@
-From actris.logrel Require Import types subtyping.
+From actris.logrel Require Import ltyping types subtyping.
 From actris.channel Require Import channel.
 From iris.base_logic.lib Require Import invariants.
 From iris.proofmode Require Import tactics.
-From iris.heap_lang Require Import proofmode.
+From iris.heap_lang Require Import notation proofmode.
+From iris.bi.lib Require Export core.
+
+(* TODO: Coq fails to infer what the Σ should be if I move some of these
+definitions out of the section or into a different section with its own Context
+declaration. *)
 
 Section copying.
   Context `{heapG Σ, chanG Σ}.
   Implicit Types A : lty Σ.
   Implicit Types S : lsty Σ.
 
+  (* We define the copyability of semantic types in terms of subtyping. *)
   Definition copyable (A : lty Σ) : iProp Σ :=
     A <: copy A.
 
-  (* Subtyping for `copy` *)
+  (* Subtyping for `copy` and `copy-` *)
   Lemma lty_le_copy A :
     ⊢ copy A <: A.
   Proof. by iIntros (v) "!> #H". Qed.
+
+  Lemma lty_le_copy_minus A :
+    copyable A -∗ copy- A <: A.
+  Proof.
+    iIntros "#HA". iIntros (v) "!> #Hv".
+  Admitted.
 
   (* Copyability of types *)
   Lemma lty_unit_copyable :
@@ -35,6 +47,10 @@ Section copying.
     ⊢ copyable (copy A).
   Proof. iIntros (v) "!> #Hv !>". iFrame "Hv". Qed.
 
+  Lemma lty_copyminus_copyable A :
+    ⊢ copyable (copy- A).
+  Proof. iIntros (v) "!> #Hv !>". iFrame "Hv". Qed.
+
   Lemma lty_any_copyable :
     ⊢ copyable any.
   Proof. iIntros (v) "!> #Hv !>". iFrame "Hv". Qed.
@@ -47,7 +63,7 @@ Section copying.
     ⊢ copyable (mutex A).
   Proof. iIntros (v) "!> #Hv !>". iFrame "Hv". Qed.
 
-  (* Commuting rules for `copy` and other type formers *)
+  (* Rules about combining `copy` and other type formers *)
   Lemma lty_prod_copy_comm A B :
     ⊢ copy A * copy B <:> copy (A * B).
   Proof.
@@ -87,7 +103,76 @@ Section copying.
     iIntros (v) "!> Hv".
     rewrite /lty_rec {2}fixpoint_unfold.
     (* iEval (rewrite fixpoint_unfold) *)
-    (* Rewriting goes crazy here *)
+    (* TODO: Rewriting goes crazy here *)
   Admitted.
+
+  (* TODO: Get rid of side condition that x does not appear in Γ *)
+  Lemma env_split_copy Γ Γ1 Γ2 (x : string) A:
+    Γ !! x = None →
+    copyable A -∗
+    env_split Γ Γ1 Γ2 -∗
+    env_split (<[x:=A]> Γ) (<[x:=A]> Γ1) (<[x:=A]> Γ2).
+  Proof.
+    iIntros (HΓx) "#Hcopy #Hsplit". iIntros (vs) "!> HΓ".
+    iPoseProof (big_sepM_insert with "HΓ") as "[Hv HΓ]"; first by assumption.
+    iDestruct "Hv" as (v ?) "HA". iDestruct ("Hcopy" with "HA") as "#HA'".
+    iDestruct ("Hsplit" with "HΓ") as "[HΓ1 HΓ2]".
+    iSplitL "HΓ1"; iApply big_sepM_insert_2; simpl; eauto.
+  Qed.
+
+  Definition env_copy (Γ Γ' : gmap string (lty Σ)) : iProp Σ :=
+    □ ∀ vs, env_ltyped Γ vs -∗ □ env_ltyped Γ' vs.
+
+  Lemma env_copy_empty : ⊢ env_copy ∅ ∅.
+  Proof. iIntros (vs) "!> _ !> ". by rewrite /env_ltyped. Qed.
+
+  Lemma env_copy_extend x A Γ Γ' :
+    Γ !! x = None →
+    env_copy Γ Γ' -∗
+    env_copy (<[x:=A]> Γ) Γ'.
+  Proof.
+    iIntros (HΓ) "#Hcopy". iIntros (vs) "!> Hvs". rewrite /env_ltyped.
+    iDestruct (big_sepM_insert with "Hvs") as "[_ Hvs]"; first by assumption.
+    iApply ("Hcopy" with "Hvs").
+  Qed.
+
+  Lemma env_copy_extend_copy x A Γ Γ' :
+    Γ !! x = None →
+    Γ' !! x = None →
+    copyable A -∗
+    env_copy Γ Γ' -∗
+    env_copy (<[x:=A]> Γ) (<[x:=A]> Γ').
+  Proof.
+    iIntros (HΓx HΓ'x) "#HA #Hcopy". iIntros (vs) "!> Hvs". rewrite /env_ltyped.
+    iDestruct (big_sepM_insert with "Hvs") as "[HA2 Hvs]"; first done.
+    iDestruct ("Hcopy" with "Hvs") as "#Hvs'".
+    iDestruct "HA2" as (v ?) "HA2".
+    iDestruct ("HA" with "HA2") as "#HA3".
+    iIntros "!>". iApply big_sepM_insert; first done. iSplitL; eauto.
+  Qed.
+
+  (* TODO: Maybe move this back to `typing.v` (requires restructuring to avoid
+  circular dependencies). *)
+  (* Typing rule for introducing copyable functions *)
+  Lemma ltyped_rec Γ Γ' f x e A1 A2 :
+    env_copy Γ Γ' -∗
+    (<[f:=(A1 → A2)%lty]>(<[x:=A1]>Γ') ⊨ e : A2) -∗
+    Γ ⊨ (rec: f x := e) : A1 → A2.
+  Proof.
+    iIntros "#Hcopy #He". iIntros (vs) "!> HΓ /=". iApply wp_fupd. wp_pures.
+    iDestruct ("Hcopy" with "HΓ") as "HΓ".
+    iMod (fupd_mask_mono with "HΓ") as "#HΓ"; first done.
+    iModIntro. iLöb as "IH".
+    iIntros (v) "!> HA1". wp_pures. set (r := RecV f x _).
+    iDestruct ("He" $!(binder_insert f r (binder_insert x v vs))
+                  with "[HΓ HA1]") as "He'".
+    { iApply (env_ltyped_insert with "IH").
+      iApply (env_ltyped_insert with "HA1 HΓ"). }
+    destruct x as [|x], f as [|f]; rewrite /= -?subst_map_insert //.
+    destruct (decide (x = f)) as [->|].
+    - by rewrite subst_subst delete_idemp insert_insert -subst_map_insert.
+    - rewrite subst_subst_ne // -subst_map_insert.
+      by rewrite -delete_insert_ne // -subst_map_insert.
+  Qed.
 
 End copying.
