theories/logrel/ltyping.v
@@ -126,53 +126,6 @@ Section Environment.
     iApply env_split_comm. iApply env_split_left; first by assumption.
     by iApply env_split_comm.
   Qed.
-
-  (* FIXME: copy *)
-  (* (* TODO: Get rid of side condition that x does not appear in Γ *) *)
-  (* Lemma env_split_copy Γ Γ1 Γ2 (x : string) A: *)
-  (*   Γ !! x = None → *)
-  (*   LTyCopy A → *)
-  (*   env_split Γ Γ1 Γ2 -∗ *)
-  (*   env_split (<[x:=A]> Γ) (<[x:=A]> Γ1) (<[x:=A]> Γ2). *)
-  (* Proof. *)
-  (*   iIntros (Hcopy HΓx) "#Hsplit". iIntros (vs) "!> HΓ". *)
-  (*   iPoseProof (big_sepM_insert with "HΓ") as "[Hv HΓ]"; first by assumption. *)
-  (*   iDestruct "Hv" as (v ?) "#HAv". *)
-  (*   iDestruct ("Hsplit" with "HΓ") as "[HΓ1 HΓ2]". *)
-  (*   iSplitL "HΓ1"; iApply big_sepM_insert_2; simpl; eauto. *)
-  (* Qed. *)
-
-  (* TODO: Prove lemmas about this *)
-  Definition env_copy (Γ Γ' : gmap string (lty Σ)) : iProp Σ :=
-    □ ∀ vs, env_ltyped Γ vs -∗ □ env_ltyped Γ' vs.
-
-  Lemma env_copy_empty : ⊢ env_copy ∅ ∅.
-  Proof. iIntros (vs) "!> _ !> ". by rewrite /env_ltyped. Qed.
-
-  Lemma env_copy_extend x A Γ Γ' :
-    Γ !! x = None →
-    env_copy Γ Γ' -∗
-    env_copy (<[x:=A]> Γ) Γ'.
-  Proof.
-    iIntros (HΓ) "#Hcopy". iIntros (vs) "!> Hvs". rewrite /env_ltyped.
-    iDestruct (big_sepM_insert with "Hvs") as "[_ Hvs]"; first by assumption.
-    iApply ("Hcopy" with "Hvs").
-  Qed.
-
-  (* FIXME: copy *)
-  (* Lemma env_copy_extend_copy x A Γ Γ' : *)
-  (*   Γ !! x = None → *)
-  (*   Γ' !! x = None → *)
-  (*   LTyCopy A → *)
-  (*   env_copy Γ Γ' -∗ *)
-  (*   env_copy (<[x:=A]> Γ) (<[x:=A]> Γ'). *)
-  (* Proof. *)
-  (*   iIntros (HΓx HΓ'x HcopyA) "#Hcopy". iIntros (vs) "!> Hvs". rewrite /env_ltyped. *)
-  (*   iDestruct (big_sepM_insert with "Hvs") as "[HA Hvs]"; first done. *)
-  (*   iDestruct ("Hcopy" with "Hvs") as "#Hvs'". *)
-  (*   iDestruct "HA" as (v ?) "#HA". *)
-  (*   iIntros "!>". iApply big_sepM_insert; first done. iSplitL; eauto. *)
-  (* Qed. *)
 End Environment.
 
 (* The semantic typing judgement *)
